# 数分2025 作业04
## 12
#### (1) 
$$
\frac{x^2+x-2}{x^2-3x+2} = \frac{(x^2-1)(x+1)}{(x^2-1)-3(x-1)} = \frac{x+2}{x-2}\\
\therefore 
\lim_{x \to 1} \frac{x^2+x-2}{x^2-3x+2} = \lim_{x \to 1} \frac{x+2}{x-2} = -3
$$

#### (3)
$$
\sqrt{x}(\sqrt{a+x} - \sqrt{x}) - \sqrt{x} \cdot \frac{a}{\sqrt{a+x}+\sqrt{x}} 
= \frac{a}{\sqrt{\frac{a}{x}+1}+1}\\
\therefore \lim_{x \to +\infty} \sqrt{x}(\sqrt{a+x} - \sqrt{x}) 
= \lim_{x \to +\infty} \frac{a}{\sqrt{\frac{a}{x}+1}+1} = \frac{a}{2}
$$

#### (5)
$$
\frac{(1+mx)^n-(1+nx)^m}{x^2} 
= \frac{C_n^2 m^2x^2 + C_n^3 m^3 x^3 + \cdots + m^nx^n(C_m^2 n^2 x^2+C_m^3 n^3 x^3+\cdots + n^mx^m)}{x^2}\\
\therefore \lim_{x \to 0} \frac{(1+mx)^n-(1+nx)^m}{x^2} = C_n^2 m - C_m^2 n = \frac{1}{2} mn^2 - \frac{1}{2} m^2 n
$$

#### (6)
$$
\frac{2}{1-x^2} - \frac{3}{1-x^3} 
= \frac{2}{(1-x)(1+x)} - \frac{3}{(1-x)(1+x+x^2)} \\
= \frac{-2(1-x^2) + (1-x)}{(1-x)(1+x)(1+x+x^2)} 
= \frac{-2x-1}{(1+x)(1+x+x^2)}\\
\therefore \lim_{x \to 1} (\frac{2}{1-x^2} - \frac{3}{1-x^3}) = \lim_{x \to 1} \frac{-2x-1}{(1+x)(1+x+x^2)} = -\frac{1}{2}
$$

#### (7)
$$
\frac{(x+\Delta x)^n-x^n}{\Delta x} 
= \frac{C_n^1 x^{n-1} \Delta x + C_n^2 x^{n-2} \Delta x^2 + \cdots+\Delta x^n}{\Delta x} 
= C_n^1 x^{n-1} + C_n^2 x^{n-2} \Delta x+ \cdots+ \Delta x^{n-1}\\
\therefore \lim_{\Delta x \to 0} \frac{(x+\Delta x)^n-x^n}{\Delta x} 
= \lim_{\Delta x \to 0} C_n^1 x^{n-1} + C_n^2 x^{n-2} \Delta x + \cdots+ \Delta x^{n-1} 
= n \cdot x^{n-1}
$$

#### (9)
$$
\frac{\cos(x+\Delta x)-\cos x}{\Delta x} 
= \frac{\cos x \cos\Delta x-\sin x \sin \Delta x - \cos x}{\Delta x} 
= \frac{(\cos \Delta x-1)(\cos x-\sin x \sin \Delta x)}{\Delta x}\\
\therefore \lim_{\Delta x \to 0} \frac{\cos(x+\Delta x)-\cos x}{\Delta x} 
=\lim_{\Delta x \to 0}\frac{(\cos \Delta x -1)\cos x- \sin x \sin \Delta x}{\Delta x}
$$
由已知,
$$
\lim_{\Delta x \to 0} \cos \Delta x = 1 
\therefore \text{ 原式 } = \lim_{\Delta x \to 0} \frac{-\sin x \sin \Delta x}{\Delta x} \\
\because \lim_{x \to 0} \frac{\sin x}{x} = 1 \therefore \text{ 原式 } = -\sin x
$$

#### (10)
$$
设t = \sqrt[n]{1+x}\\
\frac{\sqrt[n]{1+x}-1}{x}=\frac{t-1}{t^{n-1}} 
= \frac{t-1}{(t-1)(t^{n-1}+t^{n-2}+\cdots+t+1)} 
= \frac{1}{t^{n-1}+t^{n-2}+\cdots+t+1}\\
\therefore \lim_{x \to 0} \frac{n\sqrt{1+x}-1}{x} = \lim_{t \to 1} \frac{1}{t^{n-1}+t^{n-2}+\cdots+t+1} = \frac{1}{n}
$$

## 13
#### (1)
$$
x \cot 2x = \frac{x \cos 2x}{\sin 2x},
|\cos x - 1 | = 2 \sin^2 \frac{x}{2} \leq \frac{x^2}{2}\\
\because 当x \rightarrow 0时, \frac{x^2}{2} \rightarrow 0\\
\therefore \mid \cos x - 1 \mid \rightarrow 0 \therefore \lim_{x \rightarrow 0} \cos x = 1\\
\lim_{x \rightarrow 0} x \cot 2x 
= \lim_{2x \rightarrow 0} \frac{1}{2}\frac{2x \cos 2x}{\sin 2x} = \frac{1}{2}
$$

#### (3)
$$
\frac{\sin x}{x-n\pi} = \frac{(-1)^n \sin(x-n\pi)}{x-n\pi} \\
\lim_{x \rightarrow n\pi} \frac{\sin x}{x-n\pi} 
= \lim_{x-n\pi\rightarrow 0} \frac{(-1)^n \sin(x-n\pi)}{x-n\pi} = (-1)^n
$$

#### (4)
$$
(1-x)\tan \frac{\pi}{2} x = \frac{2}{\pi} \cdot (\frac{\pi}{2}-\frac{\pi}{2}x) \frac{1}{\tan(\frac{\pi}{2}-\frac{\pi}{2}x)} 
= \frac{(\frac{\pi}{2}-\frac{\pi}{2}x)\cos(\frac{\pi}{2}-\frac{\pi}{2}x)}{\sin(\frac{\pi}{2}-\frac{\pi}{2}x)} \cdot \frac{2}{\pi} \\
\lim_{x \rightarrow 1} (1-x) \tan \frac{\pi}{2} x = \lim_{(\frac{\pi}{2}-\frac{\pi}{2}x) \rightarrow 0} \frac{(\frac{\pi}{2}-\frac{\pi}{2}x)\cos(\frac{\pi}{2}-\frac{\pi}{2}x)}{\sin(\frac{\pi}{2}-\frac{\pi}{2}x)} \cdot \frac{2}{\pi} = \frac{2}{\pi}
$$

#### (8)
$$
(1+\frac{2}{3^n})^{3^n} 
= ((1+\frac{1}{\frac{3^n}{2}})^{\frac{3^n}{2}})^2 
\quad \therefore
\lim_{n \rightarrow \infty} (1+\frac{2}{3^n})^{3^n} = e^2
$$

## 14
#### (1)
$$
f(x) = \frac{1}{1+2^{\frac{1}{x}}} 
$$
$x \rightarrow 0^{-}$时:
$$
f(x) \rightarrow 1
$$
$x \rightarrow 0^{+}$时:
$$
f(x) \rightarrow 0
$$
左右极限不等, 极限不存在。

#### (2)
$$
f(x) = \begin{cases} 
\frac{\sin x}{x},& x<0 \\
(1+x)^{\frac{1}{x}},& x>0 
\end{cases}
\quad x \rightarrow 0
$$
$x \rightarrow 0^{-}$时:
$$
f(x) \rightarrow 1
$$
$x \rightarrow 0^{+}$时:
$$
(1+\frac{1}{\frac{1}{x}})^{\frac{1}{x}} (x \rightarrow +\infty), f(x) \rightarrow e
$$
左右极限不等, 极限不存在。

## 16
通分可知, 使分子次数为0, 需要 $a=-1, b=-2$.

## 17
#### (1)
$$
\left(\frac{3x-1}{3x+1}\right)^{3x-1} 
= \frac{\left(1-\frac{2}{3x+1}\right)^{\frac{3x+1}{2}} 
\cdot (1-\frac{2}{3x+1})^{\frac{3x+1}{2}}}{\left(1-\frac{2}{3x+1}\right)^2}\\
\therefore \lim_{x \to \infty} \left(\frac{3x-1}{3x+1}\right)^{3x-1} 
= \lim_{\frac{3x+1}{2} \to \infty} \frac{\left(1-\frac{2}{3x+1}\right)^{\frac{3x+1}{2}} \cdot (1-\frac{2}{3x+1})^{\frac{3x+1}{2}}}{\left(1-\frac{2}{3x+1}\right)^2} = e^{-2}
$$ 

#### (2)
$$
设f(x)=(2-x)^{\sec \frac{\pi}{2} x},(1-x)=t\\
f(x)=\left(1+\frac{1}{\frac{1}{t}}\right)^{\frac{1}{\cos\left(\frac{\pi}{2}\cdot\frac{\pi}{2}\cdot t\right)}} 
= \left(1+\frac{1}{\frac{1}{t}}\right)^{\frac{1}{\sin\frac{\pi}{2} t}}\\
\lim_{x \to 1} (2-x)^{\sec \frac{\pi}{2} x} 
= \lim_{\frac{1}{t} \to \infty} \left(1+\frac{1}{\frac{1}{t}}\right)^{\frac{1}{\sin\frac{\pi}{2} t}}\\
\because 当 t \to 0 时, 有 \frac{\frac{\pi}{2} t}{\sin\frac{\pi}{2} t} \to 1\\ 
\therefore 原式 = \lim_{\frac{1}{t} \to \infty} \left(1+\frac{1}{\frac{1}{t}}\right)^{\frac{2}{\pi} \cdot \frac{1}{t}} = e^{\frac{2}{\pi}}
$$



#### (3)
$$
\cos(\sqrt{x})^{\frac{1}{x}},\sqrt{x} \to 0^+时, \cos\sqrt{x} \sim 1-\frac{1}{2}x\\
原式 = \lim_{x \to 0^+} (1-\frac{1}{2}x)^{\frac{1}{x}} 
= \lim_{x \to 0^+} (1-\frac{\frac{1}{2}}{x})^{\frac{2}{x} \cdot \frac{1}{2}} 
= e^{-\frac{1}{2}}
$$

#### (4)
$$
\lim_{x \to 0} (\frac{\pi+e^{\frac{1}{x}}}{1+e^{\frac{4}{x}}} + arc \tan\frac{1}{x}) 
$$
$x \rightarrow 0^{-}$时:
$$
\left(\frac{\pi+e^{\frac{1}{x}}}{1+e^{\frac{4}{x}}} + arc\tan\frac{1}{x}\right) \to (\pi-\frac{\pi}{2}) = \frac{\pi}{2}
$$
$x \rightarrow 0^{+}$时:
$$
(\frac{\pi+e^{\frac{1}{x}}}{1+e^{\frac{4}{x}}} + arc\tan\frac{1}{x}) = (\frac{\frac{\pi}{e^{\frac{1}{x}}} + 1}{\frac{1}{e^{\frac{1}{x}}} + e^{\frac{3}{x}}} + arc\tan\frac{1}{x}) = \frac{\pi}{2} 
$$
综上
$$
\lim_{x \to 0} (\frac{\pi+e^{\frac{1}{x}}}{1+e^{\frac{4}{x}}} + arc\tan\frac{1}{x}) = \frac{\pi}{2}
$$

